program examples and handler_has_type scaffold

coqsrc/Explicit/MTypeRulesExamples.v
@@ -1,5 +1,8 @@
+Require Import Utf8.
+Require Import Common.MBinder.
 Require Import Explicit.MSyntax.
 Require Import Explicit.MTypeRules.
+Require Import Coq.Strings.Ascii.
 
 Example Empty_world : world :=
 {|
@@ -16,16 +19,11 @@ Example row_equivalence_example :
   〈ew_var 1; ew_var 2; ew_var 3; ew_var 4; ew_var 5〉 ≅ 
   〈ew_var 2; ew_var 1; ew_var 3; ew_var 5; ew_var 4〉.
 Proof.
-  eapply req_select.
-  { apply row_select_tail.
-    apply row_select_head. }
-  eapply req_select.
-  { apply row_select_head. }
-  eapply req_select.
-  { apply row_select_head. }
-  eapply req_select.
-  { apply row_select_tail.
-    apply row_select_head. }
+  repeat(
+    eapply req_select;
+    repeat(
+      try (apply row_select_head);
+      apply row_select_tail)).
   eapply req_refl.
 Qed.
 
@@ -36,3 +34,65 @@ Proof.
   repeat(apply row_append_step).
   apply row_append_base.
 Qed.
+
+Inductive Example_effect : Set :=
+| IO_effect : Example_effect.
+
+Example IO_effect_operation : Set := inc (inc Empty_set).
+
+Example getc : IO_effect_operation := VZ. 
+Example putc : IO_effect_operation := VS VZ.
+
+Inductive Example_base_type : Set :=
+| bt_unit : Example_base_type
+| bt_char : Example_base_type.
+
+Example Example_world : world :=
+{|
+  w_effect_t := Example_effect;
+  w_eff_op_t := λ e, IO_effect_operation;
+  w_eff_ar   := λ _, 0;
+  w_base_t   := Example_base_type;
+  w_base_v   := λ b, match b with | bt_unit => True | bt_char => ascii end
+|}.
+
+Example Example_program := expr Example_world Empty_set Empty_set.
+
+Example print_H : Example_program.
+Proof.
+  apply e_app.
+  { apply e_value.
+    apply v_eff_op with IO_effect.
+    apply putc. }
+  { apply e_value.
+    apply v_const with bt_char.
+    apply "H"%char. }
+Defined.
+
+Example IO_0_stream_Handler (e : Example_program) : Example_program.
+Proof.
+  apply e_handle with IO_effect.
+  { apply nil. }
+  { apply e. }
+  { apply h_op.
+    { apply e_app.
+      { apply e_value.
+        apply v_var.
+        apply V2_resume. }
+      apply e_value.
+      apply v_const with bt_unit.
+      constructor. }
+    apply h_op.
+    { apply e_app.
+      { apply e_value.
+        apply v_var.
+        apply V2_resume. }
+      apply e_value.
+      apply v_const with bt_char.
+      apply "000"%char. }
+    apply h_return.
+    { apply e_value.
+      apply v_var.
+      apply VZ. } }
+Defined.
+  
